share/pulse/examples/dice/cbor/CDDL.Spec.MapGroupGen.fsti
@@ -1,0 +1,260 @@
+module CDDL.Spec.MapGroupGen
+include CDDL.Spec.Base
+module Cbor = CBOR.Spec
+module U8 = FStar.UInt8
+module U64 = FStar.UInt64
+
+let rec is_sublist_of
+  (#t: Type)
+  (l1 l2: list t)
+: Tot prop
+  (decreases l2)
+= match l1, l2 with
+  | [], _ -> True
+  | _, [] -> False
+  | a1 :: q1, a2 :: q2 ->
+    (a1 == a2 /\ q1 `is_sublist_of` q2) \/
+    l1 `is_sublist_of` q2
+
+val is_sublist_of_length
+  (#t: Type)
+  (l1 l2: list t)
+: Lemma
+  (requires (is_sublist_of l1 l2))
+  (ensures (List.Tot.length l1 <= List.Tot.length l2))
+  (decreases l2)
+  [SMTPat (is_sublist_of l1 l2)]
+
+val is_sublist_of_refl
+  (#t: Type)
+  (l: list t)
+: Lemma
+  (l `is_sublist_of` l)
+  [SMTPat (l `is_sublist_of` l)]
+
+val is_sublist_of_trans
+  (#t: Type)
+  (l1 l2 l3: list t)
+: Lemma
+  (requires (
+    is_sublist_of l1 l2 /\
+    is_sublist_of l2 l3
+  ))
+  (ensures (
+    is_sublist_of l1 l3
+  ))
+  [SMTPatOr [
+    [SMTPat (is_sublist_of l1 l2); SMTPat (is_sublist_of l2 l3)];
+    [SMTPat (is_sublist_of l1 l3); SMTPat (is_sublist_of l2 l3)];
+    [SMTPat (is_sublist_of l1 l3); SMTPat (is_sublist_of l1 l2)];
+  ]]
+
+val is_sublist_of_append_right
+  (#t: Type)
+  (l1 l2 l: list t)
+: Lemma
+  (is_sublist_of (l1 `List.Tot.append` l) (l2 `List.Tot.append` l) <==>
+    is_sublist_of l1 l2)
+  [SMTPat (is_sublist_of (l1 `List.Tot.append` l) (l2 `List.Tot.append` l))]
+
+val is_sublist_of_append_left_intro
+  (#t: Type)
+  (l l1 l2: list t)
+: Lemma
+  (requires (is_sublist_of l1 l2))
+  (ensures (is_sublist_of (l `List.Tot.append` l1) (l `List.Tot.append` l2)))
+  [SMTPat (is_sublist_of (l `List.Tot.append` l1) (l `List.Tot.append` l2))]
+
+let is_sublist_of_append_intro
+  (#t: Type)
+  (l1 l2: list t)
+  (l1' l2': list t)
+: Lemma
+  (requires (
+    is_sublist_of l1 l1' /\ is_sublist_of l2 l2'
+  ))
+  (ensures (
+    is_sublist_of (l1 `List.Tot.append` l2) (l1' `List.Tot.append` l2')
+  ))
+= assert (is_sublist_of (l1 `List.Tot.append` l2) (l1' `List.Tot.append` l2))
+
+val list_filter_is_sublist_of_intro
+  (#t: Type)
+  (f: t -> bool)
+  (l: list t)
+: Lemma
+  (ensures (List.Tot.filter f l `is_sublist_of` l))
+  (decreases l)
+  [SMTPat (List.Tot.filter f l)]
+
+let notp
+  (#t: Type)
+  (p: (t -> Tot bool))
+  (x: t)
+: Tot bool
+= not (p x)
+
+val is_sublist_of_suffix
+  (#t: Type)
+  (l1 l2: list t)
+: Lemma
+  (ensures (l2 `is_sublist_of` (l1 `List.Tot.append` l2)))
+  [SMTPat (l1 `List.Tot.append` l2)]
+
+val is_sublist_of_prefix
+  (#t: Type)
+  (l1 l2: list t)
+: Lemma
+  (ensures (l1 `is_sublist_of` (l1 `List.Tot.append` l2)))
+  [SMTPat (l1 `List.Tot.append` l2)]
+
+let cbor_map_pred (l: list (Cbor.raw_data_item & Cbor.raw_data_item)) : Tot prop =
+  List.Tot.no_repeats_p (List.Tot.map fst l)
+
+let cbor_map : Type0 = (l: list (Cbor.raw_data_item & Cbor.raw_data_item) { cbor_map_pred l })
+
+val cbor_map_is_sublist_of
+  (l1 l2: list (Cbor.raw_data_item & Cbor.raw_data_item))
+: Lemma
+  (requires
+    l1 `is_sublist_of` l2
+  )
+  (ensures cbor_map_pred l2 ==> cbor_map_pred l1)
+  [SMTPat (l1 `is_sublist_of` l2)]
+
+[@@erasable]
+val map_group : Type0
+
+val map_group_always_false : map_group
+
+val map_group_end : map_group
+
+val map_group_nop : map_group
+
+val map_group_match_item (key value: typ) : map_group
+
+let matches_map_group_entry
+  (key value: typ)
+  (x: (Cbor.raw_data_item & Cbor.raw_data_item))
+: GTot bool
+= key (fst x) && value (snd x)
+
+val map_group_equiv
+  (m1 m2: map_group)
+: Tot prop
+
+val map_group_choice (m1 m2: map_group) : map_group
+
+let map_group_zero_or_one (m: map_group) : map_group =
+  map_group_choice m map_group_nop
+
+val map_group_concat (m1 m2: map_group) : map_group
+
+val map_group_concat_equiv (m1 m2 m1' m2': map_group) : Lemma
+  (requires m1 `map_group_equiv` m1' /\
+    m2 `map_group_equiv` m2'
+  )
+  (ensures (m1 `map_group_concat` m2) `map_group_equiv` (m1' `map_group_concat` m2'))
+
+val map_group_concat_assoc (m1 m2 m3: map_group) : Lemma
+  (map_group_concat m1 (map_group_concat m2 m3) `map_group_equiv` map_group_concat (map_group_concat m1 m2) m3)
+
+val map_group_mk_cut (cut: typ) : map_group
+
+val map_group_zero_or_more
+  (m: map_group)
+: map_group
+
+let map_group_one_or_more (m: map_group) : map_group =
+  map_group_concat m (map_group_zero_or_more m)
+
+let map_group_match_item_for
+  (k: Cbor.raw_data_item)
+  (ty: typ)
+: Tot map_group
+= map_group_match_item (t_literal k) ty
+
+[@@erasable]
+noeq
+type map_group_result =
+| MapGroupFail
+| MapGroupDet of cbor_map
+| MapGroupNonDet
+
+let map_group_result_prop (l: cbor_map) (r: map_group_result) : Tot prop =
+  match r with
+  | MapGroupDet m -> m `is_sublist_of` l
+  | _ -> True
+
+val apply_map_group_det (m: map_group) (l: cbor_map) : Pure map_group_result
+  (requires True)
+  (ensures fun r -> map_group_result_prop l r)
+
+val apply_map_group_det_always_false (l: cbor_map) : Lemma
+  (apply_map_group_det map_group_always_false l == MapGroupFail)
+
+val apply_map_group_det_end (l: cbor_map) : Lemma
+  (apply_map_group_det map_group_end l == (if Nil? l then MapGroupDet l else MapGroupFail))
+
+val apply_map_group_det_nop (l: cbor_map) : Lemma
+  (apply_map_group_det map_group_nop l == MapGroupDet l)
+
+val map_group_equiv_apply_map_group_det (m1 m2: map_group) (l: cbor_map) : Lemma
+  (requires map_group_equiv m1 m2)
+  (ensures apply_map_group_det m1 l == apply_map_group_det m2 l)
+
+val apply_map_group_det_map_group_equiv (m1 m2: map_group) : Lemma
+  (requires
+    (forall l . ~ (MapGroupNonDet? (apply_map_group_det m1 l))) /\
+    (forall l . apply_map_group_det m1 l == apply_map_group_det m2 l)
+  )
+  (ensures map_group_equiv m1 m2)
+
+val apply_map_group_det_choice (m1 m2: map_group) (l: cbor_map) : Lemma
+  (match apply_map_group_det m1 l with
+  | MapGroupFail -> apply_map_group_det (m1 `map_group_choice` m2) l == apply_map_group_det m2 l
+  | MapGroupDet l1 -> apply_map_group_det (m1 `map_group_choice` m2) l == MapGroupDet l1
+  | _ -> True
+  )
+
+val apply_map_group_det_concat (m1 m2: map_group) (l: cbor_map) : Lemma
+  (match apply_map_group_det m1 l with
+  | MapGroupFail -> apply_map_group_det (m1 `map_group_concat` m2) l == MapGroupFail
+  | MapGroupDet l1 -> apply_map_group_det (m1 `map_group_concat` m2) l == apply_map_group_det m2 l1
+  | _ -> True)
+
+val apply_map_group_det_match_item_for
+  (k: Cbor.raw_data_item)
+  (ty: typ)
+  (l: cbor_map)
+: Lemma
+  (apply_map_group_det (map_group_match_item_for k ty) l == (match Cbor.list_ghost_assoc k l with
+  | None ->  MapGroupFail
+  | Some x ->
+    if ty x
+    then MapGroupDet (List.Tot.filter (notp (FStar.Ghost.Pull.pull (matches_map_group_entry (t_literal k) ty))) l)
+    else MapGroupFail
+  ))
+
+val apply_map_group_det_zero_or_more_match_item
+  (key value: typ)
+  (l: cbor_map)
+: Lemma
+  (apply_map_group_det (map_group_zero_or_more (map_group_match_item key value)) l ==
+    MapGroupDet (List.Tot.filter (notp (FStar.Ghost.Pull.pull (matches_map_group_entry key value))) l)
+  )
+
+val matches_map_group (g: map_group) (m: cbor_map) : GTot bool
+
+val matches_map_group_det (g: map_group) (m: cbor_map) : Lemma
+  (match apply_map_group_det g m with
+  | MapGroupFail -> ~ (matches_map_group g m)
+  | MapGroupDet m' -> matches_map_group g m <==> m' == []
+  | _ -> True)
+
+let t_map (g: map_group) : typ =
+  fun x -> match x with
+  | Cbor.Map m -> 
+    FStar.StrongExcludedMiddle.strong_excluded_middle (List.Tot.no_repeats_p (List.Tot.map fst m)) &&
+    matches_map_group g m
+  | _ -> false
